busy_beaver/macro_machine.dfy
@@ -1,0 +1,134 @@
+// Define macro machines as abstractions over a base Turing Machine.
+
+include "tm_spec_gen.dfy"
+include "chain_sim.dfy"
+include "parse.dfy"  // Used for testing below.
+
+abstract module BlockMacroSpecAbstract refines TMSpecGenAbstract {
+  import BaseSpec : TMSpecGenAbstract
+
+  type Symbol = seq<BaseSpec.Symbol>
+  type State = BaseSpec.State
+  datatype TM = BlockMacro(base_tm : BaseSpec.TM, block_size : nat)
+
+  function method IsHalt?(state : State) : bool { BaseSpec.IsHalt?(state) }
+  function method BlankSymbol(tm : TM) : Symbol {
+    seq(tm.block_size, n => BaseSpec.BlankSymbol(tm.base_tm))
+  }
+  function method InitState(tm : TM) : State { BaseSpec.InitState(tm.base_tm) }
+  function method HaltState(tm : TM) : State { BaseSpec.HaltState(tm.base_tm) }
+
+  function method ScoreSymbol(symbol : Symbol) : nat {
+    1 // TODO
+  }
+  function method ScoreState(state : State) : nat { 0 }
+  
+
+  datatype BoundedSimResult =
+    | InfiniteInBlock
+    | HaltedInBlock(
+      new_block : seq<BaseSpec.Symbol>,
+      new_pos : nat,
+      num_base_steps : nat
+    )
+    | ExittedBlock(
+      new_block : seq<BaseSpec.Symbol>,
+      new_state : BaseSpec.State,
+      new_dir : Dir,
+      num_base_steps : nat
+    )
+
+  method BoundedSim(base_tm : BaseSpec.TM, state : BaseSpec.State,
+                    start_tape : seq<BaseSpec.Symbol>, pos : int, dir : Dir)
+    returns (result : BoundedSimResult)
+  {
+    var num_base_steps : nat := 0;
+    print "ERROR: BoundedSim Not Implemented!\n";
+  }
+
+  method LookupTrans(tm : TM, state : State, symbol : Symbol, dir : Dir)
+    returns (trans : Transition)
+  {
+    var block : seq<BaseSpec.Symbol> := symbol;
+    var pos_in_block := match dir
+      case Right => 0
+      case Left => |block| - 1;
+    var sim_result := BoundedSim(
+      tm.base_tm, state, block, pos_in_block, dir);
+    match sim_result {
+      case InfiniteInBlock =>
+        return InfiniteTrans;
+      case HaltedInBlock(_, _, _) =>
+        // This is not 100% accurate, but good enough for scoring / step count.
+        // TODO: Keep track of exact halt location inside new_block.
+        return Transition(sim_result.new_block, Right, HaltState(tm),
+                          sim_result.num_base_steps);
+      case ExittedBlock(_, _, _, _) =>
+        return Transition(sim_result.new_block, sim_result.new_dir,
+                          sim_result.new_state,
+                          sim_result.num_base_steps);
+    }
+  }
+}
+
+module BlockMacroSpecNat refines BlockMacroSpecAbstract {
+  import BaseSpec = TMSpecGenNat
+}
+
+module ChainSimBlock refines ChainSimAbstract {
+  import opened TMSpec = BlockMacroSpecNat
+}
+
+
+// Test
+import opened ChainSimBlock
+
+method VerboseSimTM(tm_str : string, block_size : nat, num_sim_steps : nat)
+  requires block_size > 0
+{
+  var base_tm := Parse.ParseTM(tm_str);
+  var tm := BlockMacroSpecNat.BlockMacro(base_tm, block_size);
+  var i := 0;
+  var config := InitConfig(tm);
+  while i < num_sim_steps && config.Config? && config.state.RunState?
+    invariant 0 <= i <= num_sim_steps
+    decreases num_sim_steps - i
+  {
+    config := Step(tm, config);
+    PrintConfig(config);
+    if config.Config? {
+      print "Tape:  Left: ";
+      if BlockMacroSpecNat.Left in config.tape.data {
+        PrintSemiTape(config.tape.data[BlockMacroSpecNat.Left]);
+      }
+      print "  /  Right: ";
+      if BlockMacroSpecNat.Right in config.tape.data {
+        PrintSemiTape(config.tape.data[BlockMacroSpecNat.Right]);
+      }
+      print "\n";
+    }
+    i := i + 1;
+  }
+}
+
+method QuietSimTM(tm_str : string, block_size : nat, num_sim_steps : nat)
+  requires block_size > 0
+{
+  var base_tm := Parse.ParseTM(tm_str);
+  var tm := BlockMacroSpecNat.BlockMacro(base_tm, block_size);
+  var config := RunTM(tm, InitConfig(tm), num_sim_steps);
+  PrintConfig(config);
+}
+
+method Main() {
+  // 4x2 Champion
+  // VerboseSimTM("1RB1LB_1LA0LC_1RZ1LD_1RD0RA", 2, 108);
+  QuietSimTM("1RB1LB_1LA0LC_1RZ1LD_1RD0RA", 2, 1000);
+  // 5x2 Champion (Block size 3)
+  QuietSimTM("1RB1LC_1RC1RB_1RD0LE_1LA1LD_1RZ0LA", 3,       1_000);
+  QuietSimTM("1RB1LC_1RC1RB_1RD0LE_1LA1LD_1RZ0LA", 3,      10_000);
+  QuietSimTM("1RB1LC_1RC1RB_1RD0LE_1LA1LD_1RZ0LA", 3,     100_000);
+  QuietSimTM("1RB1LC_1RC1RB_1RD0LE_1LA1LD_1RZ0LA", 3,   1_000_000);
+  QuietSimTM("1RB1LC_1RC1RB_1RD0LE_1LA1LD_1RZ0LA", 3,  10_000_000);
+  QuietSimTM("1RB1LC_1RC1RB_1RD0LE_1LA1LD_1RZ0LA", 3, 100_000_000);
+}
